30/01/26

<u>Proposition 1.3</u>

Let $G$ be a group. Then:

1. There exists precisely one identity element in $G$

2. For every $a \in G$ there exists precisely one right inverse (named $b$) to $a$. And this $b$ is also a left inverse of $a$ (meaning that we also have $b * a = e$). We write $a^{-1}$ for this inverse of $a$ (or $-a$ if the group operation is $+$)

<u>Proof</u>
Suppose $e$ and $e'$ are two identity elements in $G$
$$
\begin{gather*}
\implies e * e' = e \\
\implies e * e' = e' \\
\implies e = e'
\end{gather*}
$$
These results are true because $e'$ is an identity element and $e$ is also an identity element.

Let $b$ be a right inverse of $a$, and let $c$ be a right inverse of $b$
$$
\begin{align}
\implies a *(b*c) &= a*e \\
&= a \\
\text{and } a*(b*c) &= (a*b)*c \\
&=e*c \\
&=c\\
\implies a&=c \\
\implies b*a &=b*c = e
\end{align}
$$
The first line is possible because c is the right inverse of b, and because e is the identity element, $a*e = a$

The third line comes from associativity.

<u>Proposition 1.4</u>

1. (Cancellation) if $a, b, z \in G$ and $a*z = b$ (or $z*a = z*b$), then $a = b$
2. For all $a \in G$ both the equation $a*x = b$ and $y*a = b$ have a unique solution in $g$
3. For every $a \in G$ we have a $(a^{-1})^{-1} = a$
4. For all $a,b \in G$ we have $(a*b)^{-1} = b^{-1}*a^{-1}$
5. (Exponential laws) For any $m \in \mathbb{Z}$ and $a \in G$ we define:
$$
a^m:=
\begin{cases}
\underline{a*a*\dots*a} &\text{if } m>0 \\
e &\text{if } m = 0 \\
(a^{-1})^{|m|} &\text{if } m<0
\end{cases}
$$

Rule 2 can be reworded as:
For every $a \in G$, both the map $G \to G, x$