22/10/25

## The derivative as a rate of change

The derivative $f'(x)$ is the slope of the tangent line to a function $f$ at a point $x$. There is an alternative view of the derivative as an instantaneous rate of change of $f$.

The rate of change is the amount by which $f$ changes in proportion to how $x$ changes. If we look at changing $x$ to $x + h$, then $f(x)$ changes to $f(x + h)$. The amount by which $f$ has changed is $f(x + h) - f(x)$, and taking this in proportion to how much $x$ has changed is the quotient:
$$
\frac{f(x + h) - f(x)}{(x + h) - x}
$$
This is exactly the slop of the secant line connecting the points $(x, f(x))$ and $(x + h, f(x + h))$.

As $h$ is made smaller and $x + h$ becomes close to $x$, we get a more accurate description of the rate of change of $f$ at $x$.
If take the limit as $h$ approaches 0, we get the instantaneous rate of change of $f$ at $x$.

In terms of an object moving in two dimensional space, if the path of motion is given by the function $y(t)$ then the derivative $y'(t)$ is the velocity of the object, and $y''(t)$ is the acceleration of the object.
The velocity is therefore the instantaneous rate of change of the motion of the object and the acceleration is the instantaneous rate of change of the velocity of the object.

## Chain rule

<u>Note</u>

- We can denote derivatives as:
$$
f'(x) = \frac{dy}{dx}
$$
The chain rule is a formula for taking the derivative of a composition of functions.
Suppose that $y = f \cdot g$ where $f$ and $g$ are differentiable.

First, lets say that $y = f(u)$, meaning $y$ is a function depending on a variable $u$. For $u$, we want to take $g(x)$, so now we have $y = f(g(x))$ so now $y$ is dependent on $x$.

Now we want to find the rate at which $y$ changes with respect to $x$.
The chain rule describes that:
$$
\frac{dy}{dx} = \frac{dy}{du} \cdot \frac{du}{dx}
$$

Informally, we can describe this as differentiating the function, and then multiplying it by the derivative of what is inside the function's brackets:
$$
(f \cdot g)'(x) = f'(g(x)) \cdot g'(x)
$$
This can be extended to functions which are the composite of 3 other functions. To use the chain rule on these, we use the form:
$$
\frac{dy}{dx} = \frac{du}{dx} \cdot \frac{dv}{du} \cdot \frac{dy}{dv}
$$

## Differentiating trig functions

$$
\begin{align}
\frac{d}{dx}(\sin x) &= \cos x \\
\frac{d}{dx}(\cos x) &= -\sin x \\
\frac{d}{dx}(\tan x) &= \frac{\cos x \cos x - \sin x(-\sin x)}{\cos^2x} \\
&= \frac{\cos^2x - \sin^2x}{\cos^2x} \\
&= \frac{1}{\cos^2x} \\
&= \sec^2x
\end{align}
$$
<u>Proof</u>

Remember, $\to  \sin(x + h) = \sin x \cos h + \sin h \cos x$

$$
\begin{align}
(\sin x) &= \lim_{h \to 0} \frac{\sin(x + h) - \sin(x)}{h} \\
&= \lim_{h \to 0} \frac{\sin x \cos h + \cos x \sin h - \sin x}{h} \\
&= \sin x \cdot \lim_{h \to 0} \frac{\cos h - 1}{h} + \cos x \cdot \lim_{h \to 0} \frac{sin h}{h} \\
\end{align}
$$
