19/11/25

## Integration by Partial Fractions

This method is used to find the integral of rational functions in the form:
$$
\int \frac{P(x)}{Q(x)}\ dx
$$
where $P(x)$ and $Q(x)$ are polynomials. The idea is to rewrite $\frac{P(x)}{Q(x)}$ as a sum of terms which are easier to integrate.

ex.
Find $\int \frac{x + 4}{x^2 - 5x + 6}\ dx$

To do this, we must first look at the denominator of the fraction in the integrand, $x^2 - 5x + 6$ and factorise it into $(x-3)(x-2)$. We know that since this turns into two factors, the final result can be made using two fractions, so we can write:
$$
\frac{x + 4}{(x-3)(x-2)} = \frac{A}{x-3} + \frac{B}{x-2}
$$
From this, we can cross multiply and get:
$$
\begin{align}
\frac{x + 4}{(x-3)(x-2)} 
&= \frac{A}{x-3} + \frac{B}{x-2} \\
&= \frac{A(x-2)}{(x-3)(x-2)} + \frac{B(x-3)}{(x-3)(x-2)} \\
&= \frac{A(x-2) + B(x-3)}{(x-3)(x-2)}
\end{align}
$$
Now, we can compare the coefficients within the numerators,
$$
\begin{matrix}
A(x-2) = Ax - 2A & B(x-3) = Bx - 3B \\
1 = A + B & 4 = -2A - 3B
\end{matrix}
$$
The left equation is comparing the coefficients of the $x$ terms, and the right side is comparing the constants.

$$
\begin{gather*}
1 = A + B \\
4 = -2A - 3B \\ \\

2 = 2A + 2B \\
4 = -2A - 3B \\ \\

B = -6 \\
A = 7
\end{gather*}
$$
So now we have the integral
$$
\begin{align}
\int \frac{x + 4}{(x-3)(x-2)}\ dx 
&= \int \frac{7}{(x-3)} - \frac{6}{(x-2)}\ dx \\
&= 7 \ln(x-3) - 6 \ln (x-2) + C
\end{align}
$$
