17/11/25

## Substitution

The method of substitution is the integral version of the Chain Rule. Remember that,
$$
\frac{d}{dx} (f(g(x))) = f'(g(x)) \cdot g'(x)
$$

so integrating, we get
$$
\int f'(g(x)) \cdot g'(x)\ dx = f(g(x)) + c
$$
We can rewrite this using $u = g(x)$. Then $\frac{du}{dx} = g'(x)$, or loosely, $du = g'(x)\ dx$. So we get,
$$
\begin{align}
\int f'(g(x)) \cdot g'(x)\ dx 
&= \int f'(u)\ du \text{ substituting } g'(x)\ dx \text{ for } du  \\
&= f(u) + c \\
&= f(g(x)) + c
\end{align}
$$

ex.

Find $\int e^x \sqrt{1 + e^x}\ dx$

Let $u = 1+e^x$, then $du = e^x dx$
Now we have, 
$$
\begin{align}
\int \sqrt{u}\ du 
&= \int u^{\frac{1}{2}} \\
&= \frac{2}{3}u
\end{align}
$$


